Update PropLogic example to use modern syntax
Also add another proof of completeness, following approach in
Johnstone's book and getting things like compactness as a corollary.

examples/logic/propositional_logic/PropLogicScript.sml
@@ -9,7 +9,7 @@
 
 open HolKernel boolLib Parse bossLib pred_setTheory;
 
-local open stringLib in end;
+local open stringLib string_numTheory in end;
 
 val _ = new_theory "PropLogic"
 
@@ -23,167 +23,161 @@ val prop_ss = arith_ss ++ pred_setLib.PRED_SET_ss;
 (* Useful lemmas about sets.                                                 *)
 (*---------------------------------------------------------------------------*)
 
-val SUBSET_INSERT_MONO = Q.prove
-(`!A B x. A SUBSET B ==> (x INSERT A) SUBSET (x INSERT B)`,
- RW_TAC prop_ss [SUBSET_DEF]);
+Theorem SUBSET_INSERT_MONO[local]:
+  !A B x. A SUBSET B ==> (x INSERT A) SUBSET (x INSERT B)
+Proof RW_TAC prop_ss [SUBSET_DEF]
+QED
 
-val IN_MONO = Q.prove
-(`!x s. x IN s ==> !h. x IN (h INSERT s)`,
- RW_TAC prop_ss []);
+Theorem IN_MONO[local]: !x s. x IN s ==> !h. x IN (h INSERT s)
+Proof RW_TAC prop_ss []
+QED
 
-val IMAGE_CONG = Q.prove
-(`!f1 f2 s. (!x. x IN s ==> (f1 x = f2 x)) ==> (IMAGE f1 s = IMAGE f2 s)`,
- RW_TAC prop_ss [IN_IMAGE, EXTENSION] THEN METIS_TAC[]);
+Theorem IMAGE_CONG[local]:
+  !f1 f2 s. (!x. x IN s ==> (f1 x = f2 x)) ==> (IMAGE f1 s = IMAGE f2 s)
+Proof
+ RW_TAC prop_ss [IN_IMAGE, EXTENSION] THEN METIS_TAC[]
+QED
 
-val DIFF_UNION = Q.prove
-(`!x y. y SUBSET x ==> ((x DIFF y) UNION y = x)`,
- RW_TAC prop_ss [EXTENSION,SUBSET_DEF] THEN METIS_TAC[]);
+Theorem DIFF_UNION[local]:
+  !x y. y SUBSET x ==> ((x DIFF y) UNION y = x)
+Proof RW_TAC prop_ss [EXTENSION,SUBSET_DEF] THEN METIS_TAC[]
+QED
 
-val DIFF_INTER = Q.prove
-(`!x y. (x DIFF y) INTER y = {}`,
- RW_TAC prop_ss [EXTENSION] THEN METIS_TAC[]);
+Theorem DIFF_INTER[local]: !x y. (x DIFF y) INTER y = {}
+Proof
+ RW_TAC prop_ss [EXTENSION] THEN METIS_TAC[]
+QED
 
-val lem1 = Q.prove
-(`!e s1 s2. (e INSERT s1) UNION s2 = s1 UNION (e INSERT s2)`,
- RW_TAC prop_ss [EXTENSION] THEN METIS_TAC []);
+Theorem lem1[local]:
+  !e s1 s2. (e INSERT s1) UNION s2 = s1 UNION (e INSERT s2)
+Proof RW_TAC prop_ss [EXTENSION] THEN METIS_TAC []
+QED
 
-val lem2 = Q.prove
-(`!e s1 s2. ~(e IN s1) /\ ~(e IN s2) ==>
-  ((e INSERT s1) INTER s2 = s1 INTER (e INSERT s2))`,
- RW_TAC prop_ss [EXTENSION] THEN METIS_TAC[]);
+Theorem lem2[local]:
+  !e s1 s2. ~(e IN s1) /\ ~(e IN s2) ==>
+            ((e INSERT s1) INTER s2 = s1 INTER (e INSERT s2))
+Proof RW_TAC prop_ss [EXTENSION] THEN METIS_TAC[]
+QED
 
 
 (*---------------------------------------------------------------------------*)
 (* Declare HOL datatype of propositions.                                     *)
 (*---------------------------------------------------------------------------*)
 
-val _ = Hol_datatype `prop = Var of string
-                           | False
-                           | Imp of prop => prop`;
+Datatype: prop = Var string | False | Imp prop prop
+End
 
 (*---------------------------------------------------------------------------*)
 (* Make --> into an infix representing Imp(lication).                        *)
 (*---------------------------------------------------------------------------*)
 
 val _ = set_fixity "-->" (Infixr 490);
-val _ = overload_on ("-->", ``Imp``);
+Overload "-->" = ``Imp``
 
 
 (*---------------------------------------------------------------------------*)
 (* Variables of a proposition.                                               *)
 (*---------------------------------------------------------------------------*)
 
-val Vars_def =
- Define
-   `(Vars (Var s) = {Var s}) /\
-    (Vars False = {}) /\
-    (Vars (p --> q) = (Vars p) UNION (Vars q))`;
+Definition Vars_def[simp]:
+  (Vars (Var s) = {Var s}) /\
+  (Vars False = {}) /\
+  (Vars (p --> q) = (Vars p) UNION (Vars q))
+End
 
-val IN_Vars = Q.prove
-(`!x p. x IN Vars(p) ==> ?d. x = Var d`,
- GEN_TAC THEN Induct THEN RW_TAC prop_ss [Vars_def] THEN METIS_TAC[]);
+Theorem IN_Vars[local]:
+  !x p. x IN Vars(p) ==> ?d. x = Var d
+Proof
+  Induct_on ‘p’ THEN simp[DISJ_IMP_THM]
+QED
 
-val IN_Vars = Q.prove
-(`!x p. x IN Vars(p) ==> ?d. x = Var d`,
- Induct_on `p` THEN RW_TAC prop_ss [Vars_def] THEN METIS_TAC[]);
-
-val FINITE_Vars = Q.prove
-(`!p. FINITE (Vars p)`,
- Induct THEN RW_TAC prop_ss [Vars_def]);
-
+Theorem FINITE_Vars[simp]: !p. FINITE (Vars p)
+Proof Induct THEN simp[]
+QED
 
 (*---------------------------------------------------------------------------*)
 (* Value of a proposition in an environment. Environments represented by     *)
 (* functions of type string->bool.                                           *)
 (*---------------------------------------------------------------------------*)
 
-val Value_def =
- Define
-  `(Value env (Var s) = env s) /\
-   (Value env False = F) /\
-   (Value env (p --> q) = ((Value env p) ==> (Value env q)))`;
+Definition Value_def[simp]:
+  (Value env (Var s) = env s) /\
+  (Value env False = F) /\
+  (Value env (p --> q) = ((Value env p) ==> (Value env q)))
+End
 
 (*---------------------------------------------------------------------------*)
 (* Extra variables mapped by environments do not change the result of Value. *)
 (*---------------------------------------------------------------------------*)
 
-val Value_only_on_Vars = Q.prove
-(`!p env d b.
-    ~(Var d IN Vars p) ==>
-    (Value (\x. if x=d then b else env(x)) p = Value env p)`,
- Induct THEN RW_TAC prop_ss [Value_def,Vars_def]);
+Theorem Value_only_on_Vars[local]:
+  !p env d b.
+    Var d NOTIN Vars p ==>
+    Value env(| d |-> b |) p = Value env p
+Proof
+ Induct THEN simp[combinTheory.APPLY_UPDATE_THM]
+QED
 
 
 (*---------------------------------------------------------------------------*)
 (* A tautology evaluates to T in every environment.                          *)
 (*---------------------------------------------------------------------------*)
 
-val Tautology_def =
- Define
-   `Tautology p = !env. Value env p = T`;
-
+Definition Tautology_def: Tautology p = !env. Value env p = T
+End
 
 (*---------------------------------------------------------------------------*)
 (* Define the inference system. First the axioms. Note S and K similarity.   *)
 (*---------------------------------------------------------------------------*)
 
-val Ax1_def =
- Define
-  `Ax1 p q = p --> q --> p`;
+Definition Ax1_def: Ax1 p q = p --> q --> p
+End
 
-val Ax2_def =
- Define
-  `Ax2 p q r = (p --> q --> r) --> (p --> q) --> (p --> r)`;
+Definition Ax2_def: Ax2 p q r = (p --> q --> r) --> (p --> q) --> (p --> r)
+End
 
-val Ax3_def =
- Define
-  `Ax3 p = ((p --> False) --> False) --> p`;
-
+Definition Ax3_def: Ax3 p = ((p --> False) --> False) --> p
+End
 
 (*---------------------------------------------------------------------------*)
 (* Syntactic entailment via an inductive definition.                         *)
 (*---------------------------------------------------------------------------*)
 
-val (is_thm_rules, is_thm_ind, is_thm_cases) =
- Hol_reln
-  `(!p q (H:prop set). is_thm H (Ax1 p q)) /\
-   (!p q r H. is_thm H (Ax2 p q r)) /\
-   (!p H. is_thm H (Ax3 p)) /\
-   (!p H. p IN H ==> is_thm H p) /\
-   (!H p q. is_thm H (p --> q) /\ is_thm H p ==> is_thm H q)`;
-
-val [is_thm_Ax1, is_thm_Ax2,
-     is_thm_Ax3, is_thm_inH, is_thm_MP] = CONJUNCTS is_thm_rules;
+Inductive is_thm:
+[~Ax1:]
+  (!p q (H:prop set). is_thm H (Ax1 p q)) /\
+[~Ax2:]
+  (!p q r H. is_thm H (Ax2 p q r)) /\
+[~Ax3:]
+  (!p H. is_thm H (Ax3 p)) /\
+[~inH:]
+  (!p H. p IN H ==> is_thm H p) /\
+[~MP:]
+  (!H p q. is_thm H (p --> q) /\ is_thm H p ==> is_thm H q)
+End
 
 (*---------------------------------------------------------------------------*)
 (* Make ||- into an infix representing syntactic entailment.                 *)
 (*---------------------------------------------------------------------------*)
 
 val _ = set_fixity "||-" (Infix(NONASSOC, 450));
-val _ = overload_on ("||-", ``is_thm``);
-
-(*---------------------------------------------------------------------------*)
-(* Make a "strong" version of induction on the structure of a proof.         *)
-(* Not actually used in rest of the development.                             *)
-(*---------------------------------------------------------------------------*)
-
-val is_thm_strong_ind =
- IndDefLib.derive_strong_induction (is_thm_rules, is_thm_ind);
-
+Overload "||-" = “is_thm”
 
 (*---------------------------------------------------------------------------*)
 (* An example object-logic theorem and its proof.                            *)
 (*---------------------------------------------------------------------------*)
 
-val p_Imp_p = Q.prove
-(`!H p. H ||- (p --> p)`,
+Theorem p_Imp_p:
+  !H p. H ||- (p --> p)
+Proof
   REPEAT GEN_TAC THEN
- `H ||- (Ax1 p (p --> p))`   by METIS_TAC [is_thm_rules] THEN
- `H ||- (Ax2 p (p --> p) p)` by METIS_TAC [is_thm_rules] THEN
- `H ||- ((p --> p --> p) --> (p --> p))`
-                             by METIS_TAC [is_thm_rules,Ax1_def,Ax2_def] THEN
- `H ||- Ax1 p p` by METIS_TAC [is_thm_rules] THEN
- METIS_TAC [Ax1_def,is_thm_rules]);
+  `H ||- (Ax1 p (p --> p))`   by METIS_TAC [is_thm_rules] THEN
+  `H ||- (Ax2 p (p --> p) p)` by METIS_TAC [is_thm_rules] THEN
+  `H ||- ((p --> p --> p) --> (p --> p))`
+    by METIS_TAC [is_thm_rules,Ax1_def,Ax2_def] THEN
+  `H ||- Ax1 p p` by METIS_TAC [is_thm_rules] THEN
+  METIS_TAC [Ax1_def,is_thm_rules]
+QED
 
 
 (*---------------------------------------------------------------------------*)
@@ -191,80 +185,75 @@ val p_Imp_p = Q.prove
 (* and help in many object-logic deductions.                                 *)
 (*---------------------------------------------------------------------------*)
 
-val weakening_lemma = Q.prove
-(`!G p. G ||- p ==> !H. (G SUBSET H) ==> H ||- p`,
- HO_MATCH_MP_TAC is_thm_ind
-   THEN REPEAT CONJ_TAC THENL
-   [METIS_TAC [is_thm_rules],
-    METIS_TAC [is_thm_rules],
-    METIS_TAC [is_thm_rules],
-    METIS_TAC [is_thm_rules,SUBSET_DEF],
-    METIS_TAC [is_thm_rules]]);
+Theorem WEAKENING:
+  !G H p. G ||- p ∧ G SUBSET H ==> H ||- p
+Proof
+  Induct_on ‘is_thm’ >> simp[is_thm_rules] >>
+  METIS_TAC [is_thm_rules,SUBSET_DEF]
+QED
 
-val WEAKENING = Q.prove
-(`!G H p. G ||- p /\ (G SUBSET H) ==> H ||- p`,
- METIS_TAC [weakening_lemma]);
-
-val Ded1 = Q.prove
-(`!H p q. H ||- (p --> q) ==> (p INSERT H) ||- q`,
+Theorem Ded1[local]:
+  !H p q. H ||- (p --> q) ==> (p INSERT H) ||- q
+Proof
  REPEAT STRIP_TAC THEN
  `(p INSERT H) ||- (p --> q)` by METIS_TAC[WEAKENING,SUBSET_DEF,IN_INSERT] THEN
  `(p INSERT H) ||- p` by METIS_TAC[is_thm_rules,IN_INSERT] THEN
- `(p INSERT H) ||- q` by METIS_TAC[is_thm_rules]);
+ `(p INSERT H) ||- q` by METIS_TAC[is_thm_rules]
+QED
 
-val Ded2_lemma = Q.prove
-(`!H1 q. H1 ||- q ==> !p H. (H1 = p INSERT H) ==> H ||- (p --> q)`,
- HO_MATCH_MP_TAC is_thm_ind THEN RW_TAC prop_ss [] THENL
- [METIS_TAC [is_thm_rules, Ax1_def],
-  METIS_TAC [is_thm_rules, Ax1_def],
-  METIS_TAC [is_thm_rules, Ax1_def],
-  Cases_on `q=p` THENL
-  [(* nts: (p --> p) *)
-   FULL_SIMP_TAC prop_ss [] THEN RW_TAC prop_ss [p_Imp_p],
-   (* (same as cases 1-3)*)
-   METIS_TAC [is_thm_rules, Ax1_def,IN_INSERT]],
-  `H ||- (p --> q)` by METIS_TAC [] THEN
-  `H ||- (p --> q --> q')` by METIS_TAC[] THEN REPEAT(WEAKEN_TAC is_forall) THEN
-  `H ||- ((p --> q --> q') --> (p --> q) --> (p --> q'))`
-      by METIS_TAC [is_thm_rules, Ax2_def] THEN
-  METIS_TAC [is_thm_rules]]);
+Theorem Ded2[local]:
+  !H p q. (p INSERT H) ||- q ==> H ||- (p --> q)
+Proof
+  Induct_on ‘is_thm’ >> rw[] >~
+  [‘q ∈ p INSERT H’]
+  >- (gvs[] >> metis_tac[p_Imp_p, is_thm_rules, Ax1_def]) >~
+  [‘p INSERT H ||- a --> b’, ‘p INSERT H ||- a’]
+  >- (‘H ||- p --> a --> b ∧ H ||- p --> a’ by metis_tac[] >>
+      ‘H ||- Ax2 p a b’ by simp[is_thm_rules] >>
+      irule is_thm_MP >>
+      qexists‘p --> a’ >> simp[] >>
+      irule is_thm_MP >> metis_tac[Ax2_def]) >>
+  metis_tac[Ax1_def, is_thm_rules]
+QED
 
-val Ded2 = Q.prove
-(`!H p q. (p INSERT H) ||- q ==> H ||- (p --> q)`,
- METIS_TAC [Ded2_lemma]);
-
-val DEDUCTION = Q.prove
-(`!H p q. is_thm (p INSERT H) q <=> H ||- (p --> q)`,
- METIS_TAC [Ded1, Ded2]);
+Theorem DEDUCTION:
+  !H p q. is_thm (p INSERT H) q <=> H ||- (p --> q)
+Proof METIS_TAC [Ded1, Ded2]
+QED
 
 (*---------------------------------------------------------------------------*)
 (* Applications of Deduction Thm: false implies any prop, plus some others   *)
 (*---------------------------------------------------------------------------*)
 
-val P_Imp_P = Q.prove
-(`!H p. (p INSERT H) ||- p`,
-  METIS_TAC [p_Imp_p,DEDUCTION]);
+Theorem P_Imp_P:
+  !H p. (p INSERT H) ||- p
+Proof
+  METIS_TAC [p_Imp_p,DEDUCTION]
+QED
 
-val False_Imp_P = Q.prove
-(`!H p. H ||- (False --> p)`,
- REPEAT GEN_TAC THEN
- `H ||- (Ax1 False (p --> False))`
-     by METIS_TAC [is_thm_rules,WEAKENING,SUBSET_EMPTY] THEN
-     FULL_SIMP_TAC prop_ss [Ax1_def] THEN
- `(False INSERT H) ||- ((p --> False) --> False)`
-     by METIS_TAC [DEDUCTION] THEN
- `(False INSERT H) ||- (((p --> False) --> False) --> p)`
-     by METIS_TAC [is_thm_Ax3,Ax3_def,
-                   WEAKENING,SUBSET_INSERT_RIGHT,SUBSET_REFL] THEN
- `(False INSERT H) ||- p` by METIS_TAC [is_thm_MP ] THEN
- METIS_TAC [DEDUCTION]);
+Theorem False_Imp_P:
+  !H p. H ||- (False --> p)
+Proof
+  REPEAT GEN_TAC THEN
+  `H ||- (Ax1 False (p --> False))`
+    by METIS_TAC [is_thm_rules,WEAKENING,SUBSET_EMPTY] THEN
+  FULL_SIMP_TAC prop_ss [Ax1_def] THEN
+  `(False INSERT H) ||- ((p --> False) --> False)`
+    by METIS_TAC [DEDUCTION] THEN
+  `(False INSERT H) ||- (((p --> False) --> False) --> p)`
+    by METIS_TAC [is_thm_Ax3,Ax3_def,
+                  WEAKENING,SUBSET_INSERT_RIGHT,SUBSET_REFL] THEN
+  `(False INSERT H) ||- p` by METIS_TAC [is_thm_MP ] THEN
+  METIS_TAC [DEDUCTION]
+QED
 
 (*---------------------------------------------------------------------------*)
 (* Contrapositive: (p --> q) --> (~q --> ~p)                                 *)
 (*---------------------------------------------------------------------------*)
 
-val Contrapos = Q.prove
-(`!H p q. H ||- ((p --> q) --> ((q --> False) --> (p --> False)))`,
+Theorem Contrapos:
+  !H p q. H ||- ((p --> q) --> ((q --> False) --> (p --> False)))
+Proof
  REPEAT GEN_TAC THEN
  `(p INSERT (q --> False) INSERT (p --> q) INSERT H) ||- (p --> q)`
     by METIS_TAC [DEDUCTION, p_Imp_p,WEAKENING,EMPTY_SUBSET,
@@ -279,7 +268,8 @@ val Contrapos = Q.prove
         RW_TAC prop_ss [P_Imp_P]) THEN
  `(p INSERT (q --> False) INSERT (p --> q) INSERT H) ||- False`
     by METIS_TAC [is_thm_MP] THEN
- METIS_TAC [DEDUCTION]);
+ METIS_TAC [DEDUCTION]
+QED
 
 (*---------------------------------------------------------------------------*)
 (* The following statement can also be read (more comfortably) as            *)
@@ -288,9 +278,10 @@ val Contrapos = Q.prove
 (*                                                                           *)
 (*---------------------------------------------------------------------------*)
 
-val Disj_Elim = Q.prove
-(`!H p q r.
-   H ||- ((p --> r) --> (q --> r) --> ((p --> False) --> q) --> r)`,
+Theorem Disj_Elim:
+  !H p q r.
+    H ||- ((p --> r) --> (q --> r) --> ((p --> False) --> q) --> r)
+Proof
  REPEAT GEN_TAC THEN
  `((r --> False) INSERT ((p --> False) --> q) INSERT
   (q --> r) INSERT (p --> r) INSERT H) ||- (r --> False)`
@@ -331,15 +322,17 @@ val Disj_Elim = Q.prove
     by METIS_TAC [DEDUCTION] THEN
  `(((p --> False) --> q) INSERT (q --> r) INSERT (p --> r) INSERT H) ||- r`
     by METIS_TAC [is_thm_Ax3, Ax3_def, is_thm_MP] THEN
- METIS_TAC [DEDUCTION]);
+ METIS_TAC [DEDUCTION]
+QED
 
 
 (*---------------------------------------------------------------------------*)
 (*     (p --> q) --> (~p --> q) --> q                                        *)
 (*---------------------------------------------------------------------------*)
 
-val Case_Split = Q.prove
-(`!H p q. H ||- ((p --> q) --> ((p --> False) --> q) --> q)`,
+Theorem Case_Split:
+  !H p q. H ||- ((p --> q) --> ((p --> False) --> q) --> q)
+Proof
  let val lem = Q.SPECL [`H`,`p`,`p --> False`, `q`] Disj_Elim
  in
   REPEAT GEN_TAC THEN ASSUME_TAC lem THEN
@@ -352,7 +345,8 @@ val Case_Split = Q.prove
   `(((p --> False) --> q) INSERT (p --> q) INSERT H) ||- q`
     by METIS_TAC [is_thm_MP]
   THEN METIS_TAC [DEDUCTION]
- end);
+ end
+QED
 
 (*===========================================================================*)
 (* Soundness: every theorem is a tautology. Note that we have to modify      *)
@@ -380,17 +374,11 @@ e (FULL_SIMP_TAC prop_ss [Value_def]);
 (* Previous proof revised into a single tactic invocation.                   *)
 (*---------------------------------------------------------------------------*)
 
-val Sound_lemma = Q.prove
-(`!H p. H ||- p ==> (H = {}) ==> Tautology p`,
- HO_MATCH_MP_TAC is_thm_ind
-   THEN RW_TAC prop_ss [Tautology_def, Value_def, Ax1_def, Ax2_def, Ax3_def]
-   THEN FULL_SIMP_TAC prop_ss []);
-
-val Soundness = Q.store_thm(
-  "Soundness",
-  `!p. ({} ||- p) ==> Tautology p`,
-  METIS_TAC [Sound_lemma]);
-
+Theorem Soundness: !p. ({} ||- p) ==> Tautology p
+Proof
+  Induct_on ‘is_thm’ >>
+  simp[Tautology_def, Value_def, Ax1_def, Ax2_def, Ax3_def]
+QED
 
 (*===========================================================================*)
 (* Completeness: every tautology is a theorem.                               *)
@@ -399,44 +387,48 @@ val Soundness = Q.store_thm(
 (* p will evaluate to T in the given env.                                    *)
 (*===========================================================================*)
 
-val IValue_def =
- Define
-   `IValue env p = if Value env p = T then p else (p --> False)`;
+Definition IValue_def:
+  IValue env p = if Value env p = T then p else (p --> False)
+End
 
 (*---------------------------------------------------------------------------*)
 (* Sanity check, not used later.                                             *)
 (*---------------------------------------------------------------------------*)
 
-val Value_IValue = Q.prove
-(`!p env. Value env (IValue env p) = T`,
- RW_TAC prop_ss [IValue_def,Value_def]);
+Theorem Value_IValue: !p env. Value env (IValue env p) = T
+Proof
+  RW_TAC prop_ss [IValue_def,Value_def]
+QED
 
 (*---------------------------------------------------------------------------*)
 (* Variables disjoint from those of p are not moved by IValue.               *)
 (*---------------------------------------------------------------------------*)
 
-val IValue_only_on_Vars = Q.prove
-(`!p env d b. ~(Var d IN Vars p) ==>
-               (IValue (\x. if x=d then b else env(x)) p = IValue env p)`,
- RW_TAC prop_ss [IValue_def] THEN METIS_TAC[Value_only_on_Vars]);
+Theorem IValue_only_on_Vars:
+  !p env d b. Var d NOTIN Vars p ==>
+              IValue env(| d |-> b |) p = IValue env p
+Proof
+  rw[IValue_def] THEN METIS_TAC[Value_only_on_Vars]
+QED
 
-val IMAGE_IValue_only_on_Vars = Q.prove
-(`!s env d b. ~(Var d IN s) /\ (!x. x IN s ==> ?e. x = Var e) ==>
-               (IMAGE (IValue (\x. if x=d then b else env(x))) s =
-                IMAGE (IValue env) s)`,
+Theorem IMAGE_IValue_only_on_Vars:
+  !s env d b. Var d NOTIN s /\ (!x. x IN s ==> ?e. x = Var e) ==>
+              IMAGE (IValue env(| d |-> b |)) s =
+              IMAGE (IValue env) s
+Proof
  REPEAT STRIP_TAC THEN MATCH_MP_TAC IMAGE_CONG THEN
  REPEAT STRIP_TAC THEN MATCH_MP_TAC IValue_only_on_Vars THEN
- METIS_TAC [Vars_def,IN_INSERT,NOT_IN_EMPTY,IMAGE_CONG,IValue_only_on_Vars]);
-
+ METIS_TAC [Vars_def,IN_INSERT,NOT_IN_EMPTY,IMAGE_CONG,IValue_only_on_Vars]
+QED
 
 (*---------------------------------------------------------------------------*)
 (* Important lemma (from Peter Andrews' book "To Truth Through Proof").      *)
 (*---------------------------------------------------------------------------*)
 
-val Andrews_Lemma = Q.store_thm(
- "Andrews_Lemma",
- `!p env H.
-    (Vars p) SUBSET H ==> (IMAGE (IValue env) H) ||- (IValue env p)`,
+Theorem Andrews_Lemma:
+ !p env H.
+   (Vars p) SUBSET H ==> (IMAGE (IValue env) H) ||- (IValue env p)
+Proof
  Induct THENL
  [MAP_EVERY Q.X_GEN_TAC [`s`, `env`, `H`] THEN RW_TAC prop_ss [] THEN
   FULL_SIMP_TAC prop_ss [Vars_def] THEN
@@ -476,7 +468,8 @@ val Andrews_Lemma = Q.store_thm(
    `(p INSERT (IMAGE (IValue env) H)) ||- False` by METIS_TAC [DEDUCTION] THEN
    `(p INSERT (IMAGE (IValue env) H)) ||- p'`
        by METIS_TAC [False_Imp_P,is_thm_MP]
-   THEN METIS_TAC[DEDUCTION]]]);
+   THEN METIS_TAC[DEDUCTION]]]
+QED
 
 (*---------------------------------------------------------------------------*)
 (* Proof by induction on the number of variables removed from Vars(p) to get *)
@@ -486,10 +479,11 @@ val Andrews_Lemma = Q.store_thm(
 (* provable.                                                                 *)
 (*---------------------------------------------------------------------------*)
 
-val Completeness_Lemma = Q.prove
-(`!p V. Tautology p /\ (V SUBSET (Vars p))
+Theorem Completeness_Lemma:
+  !p V. Tautology p /\ (V SUBSET (Vars p))
         ==>
-         !env. (IMAGE (IValue env) V) ||- p`,
+        !env. (IMAGE (IValue env) V) ||- p
+Proof
  REPEAT GEN_TAC THEN STRIP_TAC THEN
  `?U. (U UNION V = Vars(p)) /\ (U INTER V = {}) /\ FINITE U`
    by (Q.EXISTS_TAC `Vars(p) DIFF V` THEN
@@ -497,35 +491,32 @@ val Completeness_Lemma = Q.prove
  POP_ASSUM (fn th =>
     NTAC 3 (POP_ASSUM MP_TAC) THEN Q.ID_SPEC_TAC `V` THEN MP_TAC th) THEN
  Q.ID_SPEC_TAC `U` THEN
- HO_MATCH_MP_TAC FINITE_INDUCT THEN RW_TAC prop_ss [] THENL
- [METIS_TAC [Andrews_Lemma,IValue_def,Tautology_def],
-  `U UNION (e INSERT V) = Vars p` by METIS_TAC [lem1] THEN
-  `e IN Vars(p)` by METIS_TAC [IN_UNION, IN_INSERT] THEN
-  `(e INSERT V) SUBSET Vars p` by METIS_TAC [INSERT_SUBSET] THEN
-  `~(e IN V)`
-    by (Q.PAT_ASSUM `x INTER y = {}` MP_TAC THEN
-        RW_TAC prop_ss [EXTENSION] THEN METIS_TAC[]) THEN
-  `U INTER (e INSERT V) = {}` by METIS_TAC [lem2] THEN
-  (* finally, use IH *)
-  `!env. is_thm (IMAGE (IValue env) (e INSERT V)) p`
-    by METIS_TAC[] THEN
-  REPEAT (WEAKEN_TAC is_eq) THEN POP_ASSUM MP_TAC THEN
-  REPEAT (WEAKEN_TAC is_forall) THEN Q.PAT_ASSUM `FINITE s` (K ALL_TAC) THEN
-  Q.PAT_ASSUM `(e INSERT V) SUBSET Vars p` (K ALL_TAC) THEN STRIP_TAC THEN
+ HO_MATCH_MP_TAC FINITE_INDUCT THEN RW_TAC prop_ss [] THEN1
+  METIS_TAC [Andrews_Lemma,IValue_def,Tautology_def] THEN
+ `U UNION (e INSERT V) = Vars p` by METIS_TAC [lem1] THEN
+ `e IN Vars(p)` by METIS_TAC [IN_UNION, IN_INSERT] THEN
+ `(e INSERT V) SUBSET Vars p` by METIS_TAC [INSERT_SUBSET] THEN
+ `~(e IN V)`
+   by (Q.PAT_ASSUM `x INTER y = {}` MP_TAC THEN
+       RW_TAC prop_ss [EXTENSION] THEN METIS_TAC[]) THEN
+ `U INTER (e INSERT V) = {}` by METIS_TAC [lem2] THEN
+ (* finally, use IH *)
+ `!env. is_thm (IMAGE (IValue env) (e INSERT V)) p`
+   by METIS_TAC[] THEN
+ REPEAT (WEAKEN_TAC is_eq) THEN POP_ASSUM MP_TAC THEN
+ REPEAT (WEAKEN_TAC is_forall) THEN Q.PAT_X_ASSUM `FINITE s` (K ALL_TAC) THEN
+ Q.PAT_X_ASSUM `(e INSERT V) SUBSET Vars p` (K ALL_TAC) THEN STRIP_TAC THEN
  `?d. e = Var(d)` by METIS_TAC [IN_Vars] THEN RW_TAC std_ss [] THEN
- `(IMAGE (IValue (\x. if x=d then T else env(x))) (Var(d) INSERT V)) ||- p`
+ `(IMAGE (IValue env(| d |-> T|)) (Var(d) INSERT V)) ||- p`
         by METIS_TAC[] THEN
- `(IMAGE (IValue (\x. if x=d then F else env(x))) (Var(d) INSERT V)) ||- p`
+ `(IMAGE (IValue env(| d |-> F|)) (Var(d) INSERT V)) ||- p`
         by METIS_TAC[] THEN
- Q.PAT_ASSUM `!env. (f env) ||- p` (K ALL_TAC) THEN
- FULL_SIMP_TAC std_ss [IMAGE_INSERT,IValue_def,Value_def] THEN
- `(Var d INSERT IMAGE (IValue(\x. if x=d then T else env x)) V) ||- p /\
-  ((Var d --> False) INSERT
-   IMAGE (IValue(\x. if x=d then F else env x)) V) ||- p`
-    by METIS_TAC [] THEN
- NTAC 2 (POP_ASSUM MP_TAC) THEN NTAC 2 (POP_ASSUM (K ALL_TAC)) THEN
+ Q.PAT_X_ASSUM `!env. (f env) ||- p` (K ALL_TAC) THEN
+ FULL_SIMP_TAC std_ss [IMAGE_INSERT,IValue_def,Value_def,
+                       combinTheory.UPDATE_APPLY] THEN
+ NTAC 2 (POP_ASSUM MP_TAC) THEN
  `!x. x IN V ==> ?e. x = Var(e)` by METIS_TAC [SUBSET_DEF,IN_Vars] THEN
- `!b. IMAGE (IValue (\x. (if x = d then b else env x))) V =
+ `!b. IMAGE (IValue env(| d |-> b |)) V =
       IMAGE (IValue env) V` by METIS_TAC [IMAGE_IValue_only_on_Vars] THEN
  RW_TAC prop_ss [] THEN
  (* Now just do a little object logic proof. *)
@@ -534,16 +525,255 @@ val Completeness_Lemma = Q.prove
                     by METIS_TAC [DEDUCTION] THEN
  `(IMAGE(IValue env) V) ||- ((Var d --> p) --> ((Var d --> False) --> p) --> p)`
      by METIS_TAC [Case_Split] THEN
- METIS_TAC [is_thm_MP]]);
-
+ METIS_TAC [is_thm_MP]
+QED
 
 (*---------------------------------------------------------------------------*)
 (* Completeness is then an easy consequence.                                 *)
 (*---------------------------------------------------------------------------*)
 
-val Completeness = Q.store_thm(
- "Completeness",
- `!p. Tautology p ==> {} ||- p`,
- METIS_TAC [EMPTY_SUBSET,IMAGE_EMPTY,Completeness_Lemma]);
+Theorem Completeness: !p. Tautology p ==> {} ||- p
+Proof METIS_TAC [EMPTY_SUBSET,IMAGE_EMPTY,Completeness_Lemma]
+QED
+
+(* ----------------------------------------------------------------------
+    Johnstone's approach, from "Notes on Logic and Set Theory"; showing
+    that every consistent set has a maximal (complete), consistent
+    extension.
+   ---------------------------------------------------------------------- *)
+
+Definition entails_def:
+  entails A p ⇔
+    ∀env. (∀a. a ∈ A ⇒ Value env a) ⇒ Value env p
+End
+
+Theorem entails_EMPTY:
+  entails {} p ⇔ Tautology p
+Proof
+  simp[entails_def, Tautology_def]
+QED
+
+Theorem entails_False[simp]:
+  entails Γ False ⇒ ∀env. ∃a. a ∈ Γ ∧ ¬Value env a
+Proof
+  simp[entails_def]
+QED
+
+Definition consistent_def:
+  consistent Γ ⇔ ¬(Γ ||- False)
+End
+
+Overload Not = “λp. p --> False”
+
+Theorem adequacy_implies_completeness:
+  (∀Γ. entails Γ False ⇒ ¬consistent Γ) ⇒
+  ∀Γ t. entails Γ t ⇒ Γ ||- t
+Proof
+  rpt strip_tac >>
+  ‘entails (Not t INSERT Γ) False’
+    by (gs[entails_def, SF DNF_ss] >> metis_tac[]) >>
+  ‘¬consistent (Not t INSERT Γ)’ by simp[] >>
+  WEAKEN_TAC is_forall >>
+  gs[consistent_def, DEDUCTION] >>
+  metis_tac[Ax3_def, is_thm_MP, is_thm_Ax3]
+QED
+
+(* need to be able to enumerate the props *)
+Definition prop2num_def[simp]:
+  prop2num False = 0 ∧
+  prop2num (Var s) = 2 * s2n s + 1 ∧
+  prop2num (Imp p1 p2) = 2 * (prop2num p1 *, prop2num p2) + 2
+End
+
+Definition num2prop_def:
+  num2prop n = if n = 0 then False
+               else if ODD n then Var (n2s ((n - 1) DIV 2))
+               else Imp (num2prop (nfst ((n - 2) DIV 2)))
+                        (num2prop (nsnd ((n - 2) DIV 2)))
+Termination
+  WF_REL_TAC ‘$<’ >> rw[]
+  >- (irule arithmeticTheory.LESS_EQ_LESS_TRANS >>
+      irule_at Any numpairTheory.nfst_le >> simp[arithmeticTheory.DIV_LT_X]) >>
+  irule arithmeticTheory.LESS_EQ_LESS_TRANS >>
+  irule_at Any numpairTheory.nsnd_le >> simp[arithmeticTheory.DIV_LT_X]
+End
+
+Theorem prop2num_num2prop[simp]:
+  ∀n. prop2num (num2prop n) = n
+Proof
+  recInduct num2prop_ind >> rpt strip_tac >>
+  ONCE_REWRITE_TAC [num2prop_def] >> rw[]
+  >- gs[arithmeticTheory.ODD_EXISTS, arithmeticTheory.ADD1] >>
+  gs[arithmeticTheory.EVEN_EXISTS, GSYM arithmeticTheory.EVEN_ODD] >>
+  rename [‘2 * m - 2’] >> Cases_on ‘m’ >>
+  gvs[arithmeticTheory.ADD1, arithmeticTheory.LEFT_ADD_DISTRIB]
+QED
+
+Theorem num2prop_prop2num[simp]:
+  ∀p. num2prop (prop2num p) = p
+Proof
+  Induct >> simp[] >> ONCE_REWRITE_TAC[num2prop_def] >>
+  rw[arithmeticTheory.ODD_ADD, arithmeticTheory.ODD_MULT]
+QED
+
+Theorem num2prop_11[simp]:
+  num2prop n1 = num2prop n2 ⇔ n1 = n2
+Proof
+  metis_tac[prop2num_num2prop]
+QED
+
+Theorem prop2num_11[simp]:
+  prop2num p1 = prop2num p2 ⇔ p1 = p2
+Proof
+  metis_tac[num2prop_prop2num]
+QED
+
+Definition limitbuild_def[simp]:
+  limitbuild A 0 = A ∧
+  limitbuild A0 (SUC n) =
+  let A = limitbuild A0 n;
+      p = num2prop n
+  in
+    if consistent (p INSERT A) then p INSERT A
+    else Not p INSERT A
+End
+
+Theorem limitbuild_mono:
+  ∀m n. m ≤ n ⇒ limitbuild A m ⊆ limitbuild A n
+Proof
+  simp[PULL_EXISTS, arithmeticTheory.LESS_EQ_EXISTS] >>
+  Induct_on ‘p’ >> simp[arithmeticTheory.ADD_CLAUSES] >>
+  rw[] >> gs[SUBSET_DEF]
+QED
+
+Theorem consistent_INSERT:
+  consistent A ∧ ¬consistent (a INSERT A) ⇒
+  consistent (Not a INSERT A)
+Proof
+  simp[consistent_def] >> rpt strip_tac >>
+  gs[DEDUCTION] >> metis_tac[is_thm_MP]
+QED
+
+Theorem limitbuild_preserves_consistency:
+  consistent A ⇒ ∀n. consistent (limitbuild A n)
+Proof
+  strip_tac >> Induct >> simp[] >> rw[consistent_INSERT]
+QED
+
+Theorem is_thm_FINITE_hyps:
+  ∀A a. A ||- a ⇒ ∃A0. FINITE A0 ∧ A0 ⊆ A ∧ A0 ||- a
+Proof
+  Induct_on ‘is_thm’ >> rw[] >~
+  [‘a ∈ A’] >- (qexists ‘{a}’ >> simp[is_thm_inH]) >~
+  [‘A1 ⊆ A’, ‘A1 ||- p --> q’, ‘A2 ⊆ A’, ‘A2 ||- p’]
+  >- (qexists ‘A1 ∪ A2’ >> simp[] >> irule is_thm_MP >>
+      qexists ‘p’ >> conj_tac >> irule WEAKENING >>
+      first_assum $ irule_at Any >> simp[]) >>
+  metis_tac[FINITE_EMPTY, is_thm_rules, EMPTY_SUBSET]
+QED
+
+Overload limit = “λA. BIGUNION (IMAGE (limitbuild A) UNIV)”
+
+Theorem limit_FINITE_SUBSET:
+  ∀A B. B ⊆ limit A ∧ FINITE B ⇒ ∃n. B ⊆ limitbuild A n
+Proof
+  Induct_on ‘FINITE’ >> simp[PULL_EXISTS] >> rw[] >>
+  first_x_assum $ drule_then strip_assume_tac >>
+  rename [‘B ⊆ limitbuild A n1’, ‘e ∈ limitbuild A n2’] >>
+  qexists ‘MAX n1 n2’ >> conj_tac >~
+  [‘B ⊆ limitbuild A (MAX n1 n2)’]
+  >- (irule SUBSET_TRANS >> irule_at Any limitbuild_mono >>
+      first_assum $ irule_at Any >> simp[]) >>
+  irule (iffLR SUBSET_DEF) >> first_assum $ irule_at Any >>
+  irule limitbuild_mono >> simp[]
+QED
+
+Theorem limit_consistency:
+  consistent A ⇒ consistent (limit A)
+Proof
+  simp[consistent_def] >> rpt strip_tac >>
+  ‘∃B. FINITE B ∧ B ⊆ limit A ∧ B ||- False’ by metis_tac[is_thm_FINITE_hyps] >>
+  ‘¬(B ⊆ A)’ by metis_tac[WEAKENING] >>
+  drule_all_then (qx_choose_then ‘N’ strip_assume_tac) limit_FINITE_SUBSET >>
+  ‘¬(limitbuild A N ||- False)’
+    by metis_tac[limitbuild_preserves_consistency, consistent_def] >>
+  metis_tac[WEAKENING]
+QED
+
+Theorem limits_complete:
+  ∀p. p ∈ limit A ∨ Not p ∈ limit A
+Proof
+  simp[PULL_EXISTS] >> CCONTR_TAC >> gs[] >>
+  rpt $ first_x_assum $ qspec_then ‘SUC $ prop2num p’ mp_tac >>
+  simp[limitbuild_def] >> rw[]
+QED
+
+Theorem limits_extend:
+  A ⊆ limit A
+Proof
+  simp[SUBSET_DEF, PULL_EXISTS] >> rpt strip_tac >> qexists ‘0’ >> simp[]
+QED
+
+Theorem consistent_no_False:
+  consistent A ⇒ False ∉ A
+Proof
+  simp[consistent_def] >> rpt strip_tac >> metis_tac[is_thm_inH]
+QED
+
+Theorem limit_entailed:
+  consistent (limit A) ⇒
+  ∀a. Value (λv. Var v ∈ limit A) a ⇔ a ∈ limit A
+Proof
+  strip_tac >> Induct >> qabbrev_tac ‘L = limit A’ >> simp[PULL_EXISTS]
+  >- simp[consistent_no_False] >>
+  rename [‘a --> b’] >>
+  map_every Cases_on [‘a ∈ L’, ‘b ∈ L’] >> gs[] >> CCONTR_TAC >> gs[] >~
+  [‘a ∈ L’, ‘b ∈ L’, ‘a --> b ∉ L’]
+  >- (‘Not (a --> b) ∈ L’ by metis_tac [limits_complete] >>
+      ‘L ||- b’ by metis_tac[is_thm_inH] >>
+      ‘L ||- b --> a --> b’ by metis_tac[is_thm_Ax1, Ax1_def] >>
+      ‘L ||- a --> b’ by metis_tac[is_thm_MP] >>
+      metis_tac [consistent_def, is_thm_rules]) >~
+  [‘a ∈ L’, ‘b ∉ L’, ‘a --> b ∈ L’]
+  >- (‘L ||- b’ by metis_tac[is_thm_rules] >>
+      metis_tac[consistent_def, is_thm_rules, limits_complete]) >~
+  [‘a ∉ L’, ‘b ∈ L’, ‘a --> b ∉ L’]
+  >- (‘L ||- b’ by metis_tac[is_thm_rules] >>
+      ‘L ||- a --> b’ by metis_tac[is_thm_rules, Ax1_def] >>
+      metis_tac[consistent_def, limits_complete, is_thm_rules]) >~
+  [‘a ∉ L’, ‘b ∉ L’, ‘a --> b ∉ L’]
+  >- (‘L ||- a --> b’ suffices_by
+        metis_tac[limits_complete, consistent_def, is_thm_rules] >>
+      simp[GSYM DEDUCTION] >> irule is_thm_MP >>
+      qexists ‘False’ >> simp[False_Imp_P] >> irule is_thm_MP >>
+      qexists ‘a’ >> metis_tac[IN_INSERT, is_thm_rules, limits_complete])
+QED
+
+Theorem adequacy:
+  ∀Γ. entails Γ False ⇒ ¬consistent Γ
+Proof
+  rpt strip_tac >> drule_then assume_tac limit_consistency >>
+  drule entails_False >> simp[] >> qexists ‘(λv. Var v ∈ limit Γ)’ >>
+  qx_gen_tac ‘a’ >> Cases_on ‘a ∈ Γ’ >> simp[Excl "IN_BIGUNION"] >>
+  metis_tac[limit_entailed, SUBSET_DEF, limits_extend]
+QED
+
+Theorem completeness_again:
+  entails Γ ϕ ⇒ Γ ||- ϕ
+Proof
+  metis_tac[adequacy_implies_completeness, adequacy]
+QED
+
+Theorem soundness_again:
+  Γ ||- ϕ ⇒ entails Γ ϕ
+Proof
+  Induct_on ‘is_thm’ >> simp[Ax1_def, Ax2_def, Ax3_def, entails_def]
+QED
+
+Theorem compactness:
+  entails Γ ϕ ⇒ ∃Γ₀. FINITE Γ₀ ∧ Γ₀ ⊆ Γ ∧ entails Γ₀ ϕ
+Proof
+  metis_tac[is_thm_FINITE_hyps, completeness_again, soundness_again]
+QED
 
 val _ = export_theory()
